\chapter{Calculus in Flat Geometries}

So far, we have been concerned with special relativity at a single point in spacetime.
We move now toward the description of \emph{fields} --- quantities extending across regions of spacetime.
The first step in this direction is the calculus of \emph{flat spacetime}.
In a flat geometry, we may assume that
\begin{itemize}
	\item points in spacetime are elements of a vector space, with differences of points being physically meaningful; and that
	\item fields are parametric functions of a single vector argument representing a location in spacetime.
\end{itemize}
We reserve the word \textdef{field} to mean a map with a fixed vector space codomain.
For instance, the electromagnetic bivector \emph{field} in flat space $F : \RR^4 → \EA[2]{\RR^4}$ is a function between fixed vector spaces.
In particular, the values of such a vector field at different points in spacetime belong to the same space, and for example, their sum $F(x) + F(y) ∈ A$ is well-defined.

These assumptions are acceptable in special relativity, but in arbitrary regions of spacetime and in the presence of gravity, curvature prevents spacetime from admitting a meaningful vector space structure.
It is then \emph{un-physical} to compare field values at different points in spacetime.
(Consideration of curvature leads to differential geometry and comprises \cref{part:2}.)

This chapter introduces the \emph{exterior} and \emph{vector derivatives} as instances of the `algebraic derivative' in the exterior and geometric algebras, respectively.
These devices combine derivative information with the geometrical structure inherent in the respective algebras.
To demonstrate their utility, a case study of Maxwell's equations of electromagnetism is given in terms of these algebraic derivatives.


\section{Differentiation}
\label{sec:algder}

The directional derivative of a vector field $F : V → A$ in the direction $𝒖 ∈ V$ at $𝒙 ∈ V$ may be defined in the usual way,
\begin{align}
	% ∂_𝒖 F(x) = \lim_{ε → 0}\frac{F(x + ε𝒖) - F(x)}{ε}
	∂_𝒖 F(𝒙) = \dv{ε} \eval{F(𝒙 + ε𝒖)}_{ε = 0}
	= \lim_{ε → 0}\frac{F(𝒙 + ε𝒖) - F(𝒙)}{ε}
.\end{align}
The directional derivative is linear in both its argument and direction.\sidenote{
	By a change of variables,
	\begin{math}
		∂_{u^a\ve_a}
		= \dv{ε} \eval{F(x + εu^a\ve_a)}_{ε = 0}
		= u^a \dv{\bar ε} \eval{F(x + \bar ε\ve_a)}_{\bar ε = 0}
		= u^a ∂_{\ve_a}
	\end{math}
	(summation on $a$).
}
We define the notation $∂_a ≔ ∂_{\ve_a}$ for brevity, so long as it is understood that this is not a partial derivative with respect to a scalar coordinate, $\pdv{x^a}$.
Of course, it may be viewed as such by setting $f(\etc{x^\i},n) = f(x^i\ve_i)$ so that
\begin{align}
	∂_{\ve_a}f(x^i\ve_i) = \pdv{x^a}f(\etc{x^\i},n)
,\end{align}
though this is a basis-dependent definition.


Suppose $F : V → A$ is some algebra--valued field.
It is useful to define a kind of ``total'' derivative $\DD F$ which does not depend on a direction $𝒖$, but instead encompasses, in a sense, all directional derivatives in a single object $\DD F : V → A$.
The motivation for this is that the soon-to-be-defined exterior derivative (of exterior algebra) and vector derivative (of geometric algebra) are realised as special cases of such a construction.
The derivative $\DD$ will be defined whenever there is a canonical inclusion $ι : V^* → A$ of dual vectors into the algebra, which is automatic if $A$ is a quotient of $\TA{(V^*)}$.

\begin{definition}
	\label{def:algder}
	Let $F : V → A$ be a field with values in an algebra $A$ with product $⊛$, equipped with an inclusion $ι : V^* → A$.
	The \textdef{algebraic derivative} of $F$ is
	\begin{align}
		\label{eqn:algder}
		\DD F ≔ ι(\ve^a) ⊛ ∂_{\ve_a} F
	\end{align}
	(summation on $a$) where $\set{\ve_a} ⊂ V$ and $\set{\ve^a} ⊂ V^*$ are dual bases.
\end{definition}

To understand this definition, consider the simple case of the free tensor algebra $F : V → \TA{(V^*)}$.
We leave the canonical inclusion $ι : V^* → \TA{(V^*)}$ implicit.
Given a basis $\set{\ve^a} ⊂ V^*$, the algebraic derivative is
\begin{math}
	\DD F = \ve^a ⊗ ∂_a F
,\end{math}
which simply encodes the partial derivatives of a $k$-vector $F$ in a $(k + 1)$-grade object.
In component language,
\begin{math}
	(\DD F)_{a\etc{a_\i}{}k} = ∂_aF_{\etc{a_\i}{}k}
.\end{math}

\subsection{The exterior derivative}
\label{sec:exterior-derivative-forms}

Consider a vector field $F : V → \EA{V^*}$ with values in the (dual) exterior algebra.
In this case \cref{eqn:algder} is the \textdef{exterior derivative}
\begin{align}
	\dd F = \ve^a ∧ ∂_a F
,\end{align}
where $\set{\ve^a} ⊂ V^*$ also form a basis of $\EA{V^*}$ (so $ι : V^* → \EA{V^*}$ may be omitted).
If $F : V → \EA[k]{V^*}$ is a $k$-vector field, then
\begin{math}
	\dd F = ∂_a F_{\etc{a_\i}{}k} \ve^a ∧ \etc{\ve^{a_\i}}∧k
\end{math}
is a $(k + 1)$-vector.

Using the equivalence of $\EA{V^*}$ with the subspace of antisymmetric tensors (see \cref{sec:exterior-algebra-as-antisymmetric}), the exterior derivative is seen to be the totally anti-symmetrised partial derivative.
In components,
\begin{math}
	(\dd F)_{\etc{a_\i}{}k} = ∂_{[a_1}F_{\etc[2]{a_\i}{}k]}
.\end{math}

The treatment of exterior forms is identical.
An exterior form field $φ : V → \forms[k](V, U)$ is called a $U$-valued \textdef{exterior differential $k$-form}, with exterior derivative formally defined by its action on vectors,
\begin{align}
	(\dd φ)(𝒖_0, \etc{𝒖_\i},{k})
	&= (\ve^a ∧ ∂_a φ)(𝒖_0, \etc{𝒖_\i},k)
\\	&= \frac1{k!} \sum_{σ ∈ S_{k + 1}} (-1)^σ \ve^a(𝒖_{σ(0)}) \, ∂_a φ(\etc{𝒖_{σ(\i)}}{}k)
\\	&= \sum_{i = 0}^k (-1)^i \, ∂_{𝒖_{i}} φ(𝒖_0, ..., \widehat{𝒖_i}, ..., 𝒖_k)
,\end{align}
under the Spivak convention (see \cref{sec:exterior-forms}).
Note that the directional derivative acts on the position dependence of $φ$ only --- the vectors $𝒖_i ∈ V$ are \emph{fixed} input vectors to the field $\dd φ$.
This changes when generalising to forms defined on a \emph{manifold}, where correction terms are needed to account for partial derivatives of input vectors (discussed in \cref{part:2}).


\subsection{The vector derivative}

The algebraic derivative in the tensor and exterior algebras are somewhat uninteresting because they are easily expressible in component form (e.g., $∂_aF_{\etc{a_\i}{}k}$ or $∂_{[a}F_{\etc{a_\i}{}k]}$).
This is not possible in the geometric algebra, however, because $\GA(V, η)$ is not $\ZZ$-graded, and we would face the problem of notating inhomogeneous objects with a variable number of indices.
The algebraic derivative is, however, still geometrically significant and extremely useful in geometric algebra.

In $\GA(V, η)$, the algebraic derivative is called the \textdef{vector derivative}, denoted $\vd$.
Explicitly, if $F : V → \GA(V, η)$ is a multivector field, then from \cref{eqn:algder} we take $⊛$ to be with the geometric product and take the inclusion to be\sidenote{
	We could just as well consider fields $V → \GA(V^*, η)$, avoiding the need for the isomorphism $\sharp : V^* → V$.
	But the metric is already defined, and we prefer to think about multivectors over `dual multivectors'.
}
\begin{math}
	V^* ∋ 𝒖 ↦ ι(𝒖^\sharp) ∈ \GA(V, η)
.\end{math}
Here, we use the canonical inclusion $ι : V ≡ \GA[1](V, η) → \GA(V, η)$ and the metric relating $V^* → V$.
The vector derivative is then
\begin{align}
	\vd F = \ve^a \, ∂_{\ve_a} F
\end{align}
(summation on $a$) where $\set{\ve_a} ⊂ V$ and $\set{\ve^a} ⊂ V^*$ are dual bases, and juxtaposition denotes the geometric product.
If $F$ is a homogeneous $k$-vector, then we may write its components as
\begin{math}
	F = F_{\etc{a_\i}{}k} \etc{\ve^{a_\i}}∧k
\end{math}
and hence
\begin{align}
	\vd F = ∂_{\ve^a}F_{\etc{a_\i}{}k} \, \ve^a(\etc{\ve^{a_\i}}∧k)
.\end{align}
Note that these terms are not $(k + 1)$-blades, but geometric products of vectors $\ve^a$ with $k$-blades --- in general, $(k ± 1)$-multivectors.

We may regard the vector derivative itself as an operator-valued vector,
\begin{align}
	\vd = \ve^a ∂_a
,\end{align}
reflecting the fact that $\vd$ behaves algebraically like a vector.
For instance, the derivative of a vector $𝒖$ has scalar and bivector parts,
\begin{math}
	\vd 𝒖 = \vd \fatdot 𝒖 + \vd ∧ 𝒖
,\end{math}
just like the geometric product of two vectors, $𝒖𝒗 = 𝒖 \fatdot 𝒗 + 𝒖 ∧ 𝒗$.
For a general multivector $F$, then, we have
\begin{align}
	\vd F = \vd \lcontr F + \vd ∧ F
.\end{align}
The $(k + 1)$-grade part $\vd ∧ F$ is the \emph{curl} of $F$, and coincides with the exterior derivative $\dd F$.
The $(k - 1)$-grade part involves the metric, and can be related to the `interior' derivative ${\star}{\dd}{\star} A$ via Hodge duality.\sidenote{
	Observe that
	\begin{math}
		\vd \lcontr A = \grade[k - 1]{\vd \vol^{-1}\vol A} = ±\vol\grade[1 + n - k]{\vd (\vol A)} = ± (\vol \vd) ∧ (\vol A)
	.\end{math}
}
Indeed, using \cref{eqn:geoprod-in-ea}, the vector derivative may be emulated in the exterior algebra by the combination
\begin{align}
	\vd F ≡ (-1)^s \star \dd \star F + \dd F
.\end{align}

\section{Case Study: Maxwell's Equations}


Expressed in the standard vector calculus of $\RR^3$, Maxwell's equations for the electric $\vb E$ and magnetic $\vb B$ fields in the presence of a source are
\begin{align}
	∇ \cdot \vb E &= \frac{ρ}{ε_0} &&\text{(Gauß' law)}
\\	∇ \cdot \vb B &= 0 &&\text{(Absence of magnetic monopoles)}
\\[1ex]	∇ × \vb E &= -∂_t \vb B &&\text{(Faraday's law)}
\\[1ex]	∇ × \vb B &= μ_0(\vb J + ε_0∂_t \vb E) &&\text{(Ampère's law)}
\end{align}
where $ρ$ is the scalar charge density and $\vb J$ the current density.
The constants $ε_0$ and $μ_0$ are the vacuum permittivity and permeability, respectively, related to the speed of light by $ε_0μ_0c^2 = 1$.



\begin{margintable}
	\footnotesize
	\begin{tabular}{cl}
		\\
		\multicolumn{2}{c}{\emph{Non-relativistic}} \\
		quantity & dimension \\
		$\vb E$ & $MQ^{-1}LT^{-2}$ \\
		$\vb B$ & $MQ^{-1}T^{-1}$ \\
		$ρ$ & $QL^{-3}$ \\
		$\vb J$ & $QT^{-1}L^{-2}$ \\
		$μ_0$ & $MQ^{-2}L$ \\
		$ε_0$ & $M^{-1}Q^2L^{-3}T^2$ \\
		$∇$, $∂_t$ & $L^{-1}$, $T^{-1}$ \\
		$c$ & $LT^{-1}$ \\
		\\
		\multicolumn{2}{c}{\emph{Relativistic}} \\
		quantity & dimension \\
		$F$ & $MQ^{-1}S^{-1}$ \\
		$J$ & $QS^{-3}$ \\
		$μ_0$, $ε_0^{-1}$ & $MQ^{-2}S$ \\
		$∂$ & $S^{-1}$ \\
		$c$ & $1$ \\
	\end{tabular}
	\caption{
		Dimensions of physical quantities in Maxwell's equations.
		$M$ is mass, $Q$ is electric charge, $T$ is duration and $L$ is length.
		In the relativistic formulation, $T$ and $L$ are unified and replaced by \emph{spacetime interval} $S$.
	}
\end{margintable}

\subsection{With tensor calculus}

The above can be expressed relativistically as eight scalar equations,
\setlength{\fboxsep}{1.4ex}
\begin{empheq}[box=\fbox]{align}
	\label{eqn:maxwells-tensor-form}
	∂_μF^{μν} &= μ_0J^ν
,&	∂_μG^{μν} &= 0
\end{empheq}
where $F^{μν} = -F^{νμ}$ is the Faraday tensor and $G^{μν}$ its Hodge dual, both encoding the electric and magnetic fields via
\begin{align}
	\label{eqn:components-of-electromagnetic-tensor}
	F^{i0} &= \frac{E^i}{c}
,&	F^{ij} &= -ε^{ijk}B_k
,&	G^{μν} &= \frac12 ε^{μν}{}_{ρσ} F^{ρσ}
% ,&	G^{μν} &= \frac12 η^{μρ}η^{νσ}ε_{ρσλυ} F^{λυ}
,\end{align}
and where $J^μ$ encodes both the static charge density $J^0 = cρ$ and current density $J^i = \vb J$.
The left of eqs.~\eqref{eqn:maxwells-tensor-form} is the \emph{source equation}, while the right is the \emph{second Bianchi identity}.
These equations assume the metric signature $\sig{+---}$, where the equivalent equations under $\sig{-+++}$ are obtained by a change of sign $F^{μν} \mapsto -F^{μν}$.



\begin{proof}
	We show how the relativistic equations \eqref{eqn:maxwells-tensor-form} reduce to the non-relativistic vector calculus equivalents.
	The $0$-component of the source equation is
	$∂_μ F^{μ0} = ∂_iE^i/c = μ_0J^0 = μ_0cρ$ implying $∇ · \vb E = ρ/ε_0$ (Gauß' law).
	The $i$-components are
	\begin{align}
		∂_0F^{0i} + ∂_jF^{ji} &= \frac1c ∂_t \qty(-\frac{E^i}{c}) - ∂_j ε^{jik} B_k = μ_0 J^i
\\		\qqtext{or} ∂_jε^{ijk}B_k &= μ_0 J^i + μ_0ε_0∂_tE^i
	,\end{align}
	which is equivalent to Ampère's law.
	The $0$-component of the Bianchi identity $∂_μG^{μ0} = 0$ is
	\begin{align}
		% \frac12 ε^{i0}{}_{μν}∂_iF^{μν}
		\frac12 ε^i{}_{jk}∂_iF^{jk}
		= -\frac12 ε^i{}_{jk}ε^{jkl}∂_iB_l
		= -∂_iB^i = 0
	,\end{align}
	which using the identity $ε_{ijk}ε^{jkl} = 2δ^l_i$ is $∇ · \vb B = 0$.
	Finally, the $i$-component gives
	\begin{align}
		0 = ∂_μG^{μi} &= \frac12ε^{μi}{}_{ρσ}∂_μF^{ρσ}
		= \frac12ε^{0i}{}_{jk}∂_0F^{jk} + ε^{ji}{}_{k0}∂_jF^{k0}
	\\	&= -\frac14ε^i{}_{jk}ε^{jkl}∂_0B_l - \frac1{2c} ε^{ijk}∂_jE_k
		= -\frac1{2c}\qty(∂_tB^i  + ε^{ijk}∂_jE_k)
	\end{align}
	yielding Faraday's law $∇ × \vb E = -∂_t \vb B$.
\end{proof}



\subsection{With exterior calculus}

It is easy to translate between exterior calculus and tensor calculus by identifying the former as the subalgebra of totally antisymmetric tensors (as in \cref{sec:exterior-algebra-as-antisymmetric}).
We will employ the Spivak convention, which in particular identifies $2$-forms with dyadic tensors via
\begin{align}
	\ve^μ ∧ \ve^ν ≡ \ve^μ ⊗ \ve^ν - \ve^ν ⊗ \ve^μ
\end{align}
where $\ve^μ$ are spacetime basis vectors (having physical dimensions of spacetime interval, $S$).
We then identify the electromagnetic bivector as
\begin{math}
	\mathcal{F} = \frac12 F_{μν} \ve^μ ∧ \ve^ν
\end{math}
(the $\frac12$ is omitted in the Kobayashi–Nomizu convention).


Since the charge density $J \sim QS^{-3}$ has dimensions of charge per spacetime $3$-volume, it is natural to interpret it as a \emph{trivector}
\begin{align}
	\mathcal{J} = J^{μνλ} \, \ve_μ ∧ \ve_ν ∧ \ve_λ ≔ J^μ \star \ve_μ = \frac1{3!}ε_{μνλα}J^α \ve^μ ∧ \ve^ν ∧ \ve^λ
\end{align}
so that the coefficients $J^{μνλ} \sim Q$ have dimensions of charge.\sidenote{
	Note that dual vectors $\ve_μ$ have dimension $S^{-1}$.
}

The relativistic Maxwell equations are then
\begin{empheq}[box=\fbox]{align}
	\dd \star \mathcal{F} &= μ_0 \mathcal{J}
,&	\dd \mathcal{F} &= 0
.\end{empheq}
\begin{proof}
	The first equation written in component form is
	\begin{align}
		\frac14 ε_{μνρσ}∂_λF^{ρσ} &= \frac1{3!}ε_{λμνα}μ_0J^α
	,\end{align}
	which, by contracting with $ε^{μνλβ}$ and using the identities
	\begin{math}
		ε^{μνλβ}ε_{μνρσ} = 2(δ^λ_ρδ^β_σ - δ^λ_σδ^β_ρ)
		\text{ and }
		ε^{μνλβ}ε_{λμνα} = 3!δ^β_σ
	,\end{math}
	reduces to
	\begin{align}
		\frac12(∂_λF^{λβ} - ∂_λF^{βλ}) &= μ_0J^β
	\end{align}
	or $∂_μF^{μν} = μ_0J^ν$, the source equation.
	The Bianchi identity can be rewritten as
	\begin{align}
		∂_μG^{μν}
		= \frac12ε^{μν}{}_{ρσ}∂_μF^{ρσ}
		= -\frac12ε^{ν[μρσ]}∂_μF_{ρσ}
		= -\frac12ε^{νμρσ}∂_{[μ}F_{ρσ]}
		= 0
	,\end{align}
	implying $\dd \mathcal{F} = 0$.
\end{proof}


\subsection{With geometric calculus}

Using the spacetime algebra $\GA(1,3)$ with vector basis $\set{\vg_μ}$ as introduced in \cref{cha:sta}, the electromagnetic bivector is\sidenote{
	This coincides with the electromagnetic bivector $2$-form $\mathcal{F}$ in the Kobayashi–Nomizu convention, because the wedge product in geometric algebra is naturally normalised (see \cref{tbl:wedge-conventions}).
}
\begin{align}
	\label{eqn:ga-em-bivector}
	F = F^{μν} \vg_μ\vg_ν
\end{align}
and the current density is
\begin{align}
	\vb J = J^μ \vg_μ
.\end{align}
Maxwell's equations are equivalent to the \emph{single} multivector equation
\begin{empheq}[box=\fbox]{align}
	\label{eqn:maxwell-sta}
	\vd F = μ_0\vb J
.\end{empheq}
\begin{proof}
	The multivector equation $\vd F = μ_0\vb J$ separates into a vector part 
	\begin{math}
		{\vd \cdot F} = μ_0\vb J
	\end{math}
	and a trivector part
	\begin{math}
		\vd ∧ F = 0
	.\end{math}
	In terms of components, the left-hand side of the vector part is
	\begin{align}
		\vd \cdot F = ∂_λF^{μν} \vg^λ \cdot (\vg_μ\vg_ν)
	,\end{align}
	whose only non-zero components are those for which $μ \ne ν$.
	If $λ$, $μ$ and $ν$ are all distinct, then $\vg^λ \cdot (\vg_μ\vg_ν) = \grade[1]{\vg^λ\vg_μ\vg_ν} = 0$.
	There are then two cases, $λ = μ$ and $λ = ν$, which respectively simplify to
	\begin{align}
		\vg^μ \cdot (\vg_μ\vg_ν) &= \grade[1]{\vg^μ\vg_μ\vg_ν} = \vg_ν
	,\\	\vg^ν \cdot (\vg_μ\vg_ν) &= \grade[1]{\vg^ν\vg_μ\vg_ν} = -\vg_μ
	,\end{align}
	so that
	\begin{align}
		\vd \cdot F = \qty(∂_μF^{μν}\vg_ν - ∂_νF^{μν}\vg_μ) = ∂_μF^{μν}\vg_ν
	.\end{align}
	Equality with the right-hand side $μ_0J^ν\vg_ν$ recovers the source equation.

	It is clear that the trivector part
	\begin{align}
		\vd ∧ F = ∂_λF^{μν} \vg^λ ∧ (\vg_μ\vg_ν) = ∂_λF_{μν} \vg^λ ∧ \vg^μ ∧ \vg^ν = 0
	\end{align}
	is equivalent to the exterior algebraic Bianchi identity $\dd \mathcal{F} = 0$.
\end{proof}


\subsubsection{In terms of electric and magnetic fields}



It is worth showing how the relativistic Maxwell equation \eqref{eqn:maxwell-sta} splits into a frame-dependent description in the geometric algebra framework.
As in \cref{sec:spacetime-split}, we use the notation $\vec u$ to indicate relative vectors; i.e., timelike bivectors
of the spacetime algebra $\GA(1,3)$ which are simultaneously grade-$1$ vectors in the observer's algebra $\GA(3)$.

From \cref{eqn:ga-em-bivector,eqn:components-of-electromagnetic-tensor}, the electromagnetic bivector is expressed in the $\vg_0$-frame as\sidenote{
	We assume $\sig{+---}$ for concreteness; for $\sig{-+++}$ replace $F \mapsto -F$.
}
\begin{align}
	\label{eqn:F-is-E-iB}
	F = \frac1c \vec E + \vol \vec B
,\end{align}
where
\begin{math}
	\vec E = E^i\vs_i = E^i \vg_i\vg_0
\end{math}
and
\begin{align}
	\vol\vec B = B_i \vol \vs^i = \frac12 B_i ε^{ijk}\vs_j\vs_k
	= \frac12 B_i ε^{ijk}\vg_j\vg_k
.\end{align}
\Cref{eqn:F-is-E-iB} should be compared with the Riemann-Silberstein vector \cite{silberstein} which has the form $\vec F_\CC = \vec E + ic\vec B$.

Similarly, the current density spacetime vector $J$ may be viewed under the space\slash time split by (left) multiplying by the frame velocity $\vg_0$,
\begin{align}
	\vg_0 \vb J = cρ - \vec J
,\end{align}
where $J^0 = cρ$ and $\vec J = J^i \vs_i$.
Similarly for the vector derivative, we have
\begin{align}
	\vg_0 \, \vd = \frac1c \pdv{t} + \vec ∇
\end{align}
in either signature.

Putting these together, the $\vg_0$-frame equation
\begin{math}
	\vg_0 \, \vd F =  μ_0 \vg_0 \vb J
\end{math}
is
\begin{align}
	\qty(\frac1c \pdv{t} + \vec ∇)\qty(\frac1c \vec E + \vol \vec B) &= μ_0\qty(cρ - \vec J)
.\end{align}
By expanding and equating grades, we obtain four equations:
\begin{align}
	\frac1c \vec ∇ · \vec E &= μ_0 cρ
&	&\text{(scalar)}
\\	\frac1{c^2} \pdv{\vec E}{t} + \vol (\vec ∇ ∧ \vec B) &= -μ_0 \vec J
&	&\text{(vector)}
\\	\frac1c \vec ∇ ∧ \vec E + \frac\vol c \pdv{\vec B}{t} &= 0
&	&\text{(bivector)}
\\	\vol (\vec ∇ · \vec B) &= 0
&	&\text{(pseudoscalar)}
\end{align}
Note that the cross product relates to the bivector curl in $\GA(3)$ by
\begin{align}
	𝒖 ∧ 𝒗 = \vol(𝒖 × 𝒗)
	\qqtext{so that}
	∇ × 𝑿 = -\vol(\vec ∇ ∧ \vec X)
.\end{align}
Hence, by adjusting by factors of $c$ and $\vol$ (and using $μ_0ε_0c^2 = 1$), the above equations reduce immediately to Gauß's law, Ampère's law, Faraday's law and the magnetic monopole equation, respectively.

The calculations in this section were performed assuming $η = \op{diag}\sig{+---}$.
In the $\sig{-+++}$ signature, $\vg_0 \vb J = -cρ + \vec J$ differs by an overall sign, which is absorbed by $F \mapsto -F$.

